Makefile
@@ -5,11 +5,9 @@ args = -impredicative-set
 all:
 	coqc $(args) init.v
 	coqc $(args) utils.v
-	coqc $(args) arity.v
 	coqc $(args) univ.v
 	coqc $(args) generic.v
 	coqc $(args) examples.v
-	coqc $(args) proofs.v
 
 clean:
 	rm *.vok *.glob *.vo *.vos
